Test/dafny0/NewtypesResolution.dfy
@@ -380,3 +380,118 @@ module CycleUnsoundnessRegression {
     assert P(x);
   }
 }
+
+// ----- cycle through function-by-method's
+
+module FunctionByMethod {
+  // --- constraints
+
+  newtype NT0 = x: int | P0(x)  // error: recursive dependency
+  predicate P0(x: int) {
+    x as NT0 == 3
+  } by method {
+    return x == 3;
+  }
+
+  newtype NT1 = x: int | P1(x)
+  predicate P1(x: int) {
+    x == 3
+  } by method {
+    return x as NT1 == 3;
+  }
+
+  type ST0 = x: int | Q0(x)  // error: recursive dependency
+  predicate Q0(x: int) {
+    x as ST0 == 3
+  } by method {
+    return x == 3;
+  }
+
+  type ST1 = x: int | Q1(x)
+  predicate Q1(x: int) {
+    x == 3
+  } by method {
+    return x as ST1 == 3;
+  }
+
+  // witnesses
+
+  newtype NW0 = x: int | true ghost witness NWitness0()  // error: recursive dependency
+  function NWitness0(): int {
+    150 + (0 as NW0 as int)
+  } by method {
+    return 150;
+  }
+
+  newtype NW1 = x: int | true ghost witness NWitness1()
+  function NWitness1(): int {
+    150
+  } by method {
+    return 150 + (0 as NW1 as int);
+  }
+
+  newtype NW2 = x: int | true witness NWitness2()  // error: recursive dependency
+  function NWitness2(): int {
+    150 + (0 as NW2 as int)
+  } by method {
+    return 150;
+  }
+
+  newtype NW3 = x: int | true witness NWitness3()  // error: recursive dependency
+  function NWitness3(): int {
+    150
+  } by method {
+    return 150 + (0 as NW3 as int);
+  }
+
+  type SW0 = x: int | true ghost witness SWitness0()  // error: recursive dependency
+  function SWitness0(): int {
+    150 + (0 as SW0 as int)
+  } by method {
+    return 150;
+  }
+
+  type SW1 = x: int | true ghost witness SWitness1()
+  function SWitness1(): int {
+    150
+  } by method {
+    return 150 + (0 as SW1 as int);
+  }
+
+  type SW2 = x: int | true witness SWitness2()  // error: recursive dependency
+  function SWitness2(): int {
+    150 + (0 as SW2 as int)
+  } by method {
+    return 150;
+  }
+
+  type SW3 = x: int | true witness SWitness3()  // error: recursive dependency
+  function SWitness3(): int {
+    150
+  } by method {
+    return 150 + (0 as SW3 as int);
+  }
+
+  // constants
+
+  ghost const c0 := R0()  // error: recursive dependency
+  function R0(): int {
+    2 + c0
+  } by method {
+    return 2;
+  }
+
+  const c1 := R1()  // error: recursive dependency
+  function R1(): int {
+    2 + c1
+  } by method {
+    return 2;
+  }
+
+  const c2 := R2()  // error: recursive dependency
+  function R2(): int {
+    2
+  } by method {
+    return 2 + c2;
+  }
+}
